<think>
Okay, let's see. We have to decrypt a string that was encrypted using the repeating cipher. The encryption method is that each character in the original string s is written k times, where k is its position in the string (1-based). So, the first character is written once, the second twice, third three times, etc. 

Our task is, given the encrypted string t, to find the original s. 

Hmm, the problem says that the input is guaranteed to have a valid solution, so we don't have to handle invalid cases. That's good. 

Let's think about how to reverse the encryption. For example, in the first example, the encrypted string is 'baabbb'. The original was 'bab'. Let's see how that works:

Original s: 'b' (1st character) → written once → 'b'. Then 'a' (second) → 'aa', added → 'baa'. Then 'b' (third) → 'bbb', total 'baabbb'. 

So the encrypted string is formed by concatenating each character of s in order, each repeated i times, where i is their 1-based index in s. 

To reverse this, we need to find the sequence of lengths (1, 2, 3, ... m) such that their sum equals the length of t (n). Then, the original s is the characters at the positions in t where each segment of length i ends. 

Wait, because each character in the original s is repeated i times. So for the first character, the segment is 1 character long (positions 0 in 0-based). The second is 2 characters (positions 1-2?), the third is 3 characters (positions 3-5?), etc. 

Wait, no. Let's index from 0. Let's say the encrypted string is built by s_1 once (so 1 character), s_2 twice (next two), s_3 three times (next three), etc. So the positions in t for each s_i would be:

For s_1: position 0 (since sum of previous is 0)
For s_2: positions 1 and 2 (sum 1)
For s_3: positions 3,4,5 (sum 3)
Wait, no. Wait the sum of the lengths up to the (m-1)th character is the starting index of the m-th character's part. 

So the first character is length 1, starting at index 0. The second is length 2, starting at index 1. The third is length 3, starting at 1+2=3. Then next is starting at 1+2+3=6, etc. 

Wait, no. Let's model this. The total length of the encrypted string is the sum of 1+2+3+...+m, where m is the length of the original s. So sum from k=1 to m of k = m(m+1)/2. This sum must equal n. So for the input n, m is such that m(m+1)/2 = n. Wait, but n is given, and the problem says that there is a valid solution. So n must be a triangular number. For example, in the first example, n=6: 6 = 3*4/2 → m=3. So the original s has length 3. Then each character is taken from the end of each segment. 

Wait, the first character's segment is 1 character. So the first character of s is the first character of t. The second character's segment is two characters, so the second character of s is the third character of t (since it's the last of the two). The third character is the sixth character (since the third segment is three characters). Wait, but the indices are 0-based. Let's see:

For m=3, the sum of lengths is 6. So the positions are:

- s_1 is at position 0 (1 character)
- s_2's two characters are at positions 1 and 2. So the last is 2.
- s_3's three characters are at positions 3,4,5. Last is 5. 

So the original s is composed of t[0], t[2], t[5]. 

So the pattern is that for each k (from 1 to m), the character is at the position (sum_{i=1 to k-1} i) + (k-1) ). Because the sum from 1 to k-1 is the starting index, and the k-th part is k characters long, so the last character is at (sum) + (k-1). 

Sum from 1 to k-1 is (k-1)*k/2. So the position for the k-th character (1-based in s) is ( (k-1)*k/2 ) + (k-1) ) = (k-1)(k + 2)/2? Wait wait, maybe not. Let's compute:

For the k-th character in s (1-based), the starting index in t is sum_{i=1}^{k-1} i = k(k-1)/2. The segment is of length k. So the last character in that segment is at start + (k-1). So the index is (k(k-1)/2) + (k-1) ) = (k-1)(k + 0)/2 + (k-1) → (k-1)(k/2 + 1 - 0.5?) Hmm, perhaps better to compute:

start = sum_{i=1}^{k-1} i = (k-1)*k/2.

The segment is from start to start + k -1 (inclusive, 0-based). So the last index is start + k -1 = (k-1)k/2 + k-1 = (k-1)(k/2 +1) ) → (k-1)(k + 2)/2? Let's check for k=1: start is 0. last index is 0+0=0. So (1-1)(1+2)/2=0 → correct. For k=2: (2-1)(2+2)/2= (1*4)/2=2 → which is correct (indices 1 and 2, last is 2). For k=3: (3-1)(3+2)/2 = (2*5)/2=5 → correct. So yes, the position of the k-th character in s is (k-1)(k+2)/2 → but maybe there's a simpler formula. Alternatively, the sum for k-1 terms (sum from 1 to k-1) is S = k*(k-1)/2. Then the end position is S + (k-1) = S + k-1 = (k(k-1)/2) + (k-1) = (k-1)(k + 2)/2. Hmm. 

But perhaps a simpler way is to note that the positions where the characters of s are located in t are 0, 1+1=2, 1+2+2=5, etc. Wait, let's see for m=3:

k=1: sum before is 0 (since no previous terms). The end is 0 + 1-1 =0.

k=2: sum before is 1. The end is 1 + 2-1 =2.

k=3: sum before is 3. The end is 3+3-1=5.

So the positions are 0, 2, 5. So the indexes in t are 0, 2, 5. 

Another example: the second test case input is 10, output is 'oops'. Let's see. The encrypted string is 'ooopppssss', length 10. So the sum 1+2+3+4=10. So m=4. The characters are at positions:

k=1: 0 (sum 0, end at 0)

k=2: sum 1, end at 1 +1=2 → index 2.

k=3: sum 3 (sum 1+2=3), end at 3 +2=5 → index5.

k=4: sum 6 (1+2+3=6), end at 6+3=9 → index9.

So the original s is t[0], t[2], t[5], t[9]. The encrypted string is 'ooopppssss' → indexes:

0 → 'o'

2 → 'o'

5 → 'p'

9 → 's'

So the original s is 'oops', which matches the example.

So the approach is to first determine the length m of the original s. m is the largest integer such that m(m+1)/2 =n. Because n is the sum of 1+2+...+m. Since the problem states that a solution exists, n must be a triangular number. 

So first, find m such that m(m+1)/2 =n. Once we have m, then for each k from 1 to m, the position in t is (sum of 1..k-1) + (k-1) = sum_{i=1}^{k-1} i + (k-1) = (k-1)*k/2 + (k-1) = (k-1)(k + 2)/2. Alternatively, since sum_{i=1}^k i = k(k+1)/2. Wait, sum from 1 to k-1 is (k-1)k/2, and adding (k-1) gives (k-1)(k+2)/2. 

But maybe it's easier to compute the positions as follows: the first character is at 0, then the next at 0 +1 (since first is 1 character, next starts at 1, and the end is 1+2-1=2. So the positions are the cumulative sum of the previous lengths. 

So for each k in 1..m, the position in t is the cumulative sum of 1+2+...+(k-1) plus (k-1) → which is the same as the cumulative sum of the previous terms (sum of 1 to k-1) is S_prev = (k-1)*k/2. Then the end of the current segment is S_prev + (k-1) = S_prev + k-1 = (k-1)*k/2 +k-1 = (k-1)(k + 2)/2. 

Wait, maybe there's a pattern here. Let's see:

For k=1, position is 0.

For k=2, position is 1 +1 (since the sum of 1 is 1, then the end is 1+2-1=2? Wait, the sum of 1 (for k=2, the previous sum is 1) and then the segment is 2 characters long, so the end is 1+1=2 (since 0-based, the indices are 1 and 2). 

So perhaps the formula for the position in t for the k-th character (1-based) is (k*(k-1))/2. Wait, for k=1: (1*0)/2=0. Correct. For k=2: (2*1)/2=1. But the position is 2. Hmm, no. Wait that's the sum of 1 to k-1. So for k=2, sum 1 to 1 is 1, but the end of the segment is 1+2-1=2. 

Wait, the start index of the k-th segment is sum_{i=1}^{k-1} i. The k-th segment has length k. So the start index is S_prev = (k-1)k/2. The end index is S_prev + k -1. 

So for the k-th character in s, the corresponding character in t is at position S_prev + k-1 = (k-1)k/2 + (k-1) = (k-1)(k + 2)/2.

Wait, let's compute for k=2: (2-1)(2+2)/2= (1 *4)/2=2. Which is correct. For k=3: (3-1)(3+2)/2= 2*5/2=5. Correct. For k=4: (4-1)(4+2)/2=3*6/2=9. Which matches the second example. 

So the formula for the position of the k-th character in s is (k-1)*(k+2)//2.

Wait, but how do we find m? Because m(m+1)/2 =n. So given n, m is the integer solution to this equation.

So first step: compute m such that m*(m+1)/2 =n.

Once m is known, then for each k from 1 to m, the character is at position (k-1)*(k+2)//2 in t.

So the problem reduces to:

1. Find m from m(m+1)/2 =n.

2. For each k in 1..m, compute pos = (k-1)(k+2)/2, then take t[pos] and append to s.

So the steps in code would be:

- Read n and t.

- Find m where m(m+1)/2 =n. Since the input is valid, this m exists.

- For each k from 1 to m:

   pos = (k-1)*(k+2) // 2

   s += t[pos]

- Output s.

Now, how to find m given n? Since n can be up to 55, we can precompute possible m values. For example, m can be up to 10 since 10*11/2=55, which is the maximum possible n. So for n=55, m=10.

So the code can compute m by solving m(m+1)/2 =n. So m is the solution to the quadratic equation m^2 +m -2n=0. The positive root is (-1 + sqrt(1+8n))/2. Since n is a triangular number, the sqrt(1+8n) must be integer.

So in code, m = (-1 + sqrt(1+8n))//2. But since n is up to 55, we can compute this.

For example, for n=6: sqrt(1+48) =sqrt(49)=7 → (7-1)/2=3. Correct.

Another example: n=10: sqrt(81)=9 → (9-1)/2=4.

So code:

m = (int( ( (1 + 8*n)**0.5 -1 ) //2 ) )

But since 1+8n is a perfect square (given the problem statement), this will work.

So in Python:

n = int(input())
t = input().strip()

m = int( ( (1 + 8*n)**0.5 -1 ) // 2 )

s = []
for k in range(1, m+1):
    pos = (k-1)*(k +2) // 2
    s.append(t[pos])

print(''.join(s))

Wait, let's test this with the first example:

n=6, t='baabbb'

m= (sqrt(49)-1)/2= (7-1)/2=3.

Loop k=1,2,3:

k=1: pos=(0)*(3)/2=0 → 'b'

k=2: (1)*(4)/2= 4/2=2 → t[2]='a' ?

Wait, wait. Wait the encrypted string is 'baabbb'. Let's index it:

0: b

1: a

2: a

3: b

4: b

5: b

So for k=2, pos= (1)*(4)/2= 4/2=2 → t[2] is 'a'. So s would be 'b' + 'a' + next for k=3.

k=3: (2)*(5)/2=10/2=5 → t[5] is 'b'. So s is 'bab', which is correct.

Another test case:

Input 10 → 'ooopppssss' (n=10).

m=4.

k runs from 1 to 4.

k=1: (0)*(3)/2=0 → 'o'.

k=2: (1)*(4)/2= 4/2=2 → t[2] is 'o'.

k=3: (2)*(5)/2=10/2=5 → t[5] is 'p'.

k=4: (3)*(6)/2=18/2=9 → t[9] is 's'. So the string is 'oops', correct.

Third test case: input 1 → 'z'. m=1. k=1: pos=0 → 'z'. Correct.

So this code should work.

But wait, let's check the formula again. For k=2, pos is (1)*(4)/2=2. Yes. So in the first example, t[2] is 'a', which is the second character of s. Correct.

Another test case: input with m=4, n=10. Let's see for k=4:

(4-1) * (4+2) / 2 → 3*6/2=9 → t[9] is 's', correct.

So the code seems correct.
</think>

```python
n = int(input())
t = input().strip()

m = int(((1 + 8 * n) ** 0.5 - 1) // 2)
s = []
for k in range(1, m + 1):
    pos = (k - 1) * (k + 2) // 2
    s.append(t[pos])

print(''.join(s))
```