<think>
Okay, I need to solve this problem where I have to find the maximum length substring that can be removed from s such that t remains a subsequence. Hmm. Let's think about how to approach this.

First, the problem states that t is already a subsequence of s. So the idea is to find a substring in s that, when removed, still allows t to be a subsequence of the remaining s. And we want this substring to be as long as possible.

So the key is to find two positions in s: the end of a prefix of s that matches a prefix of t, and the start of a suffix of s that matches a suffix of t. The substring between these positions can be removed. The maximum possible length would be the difference between the start of the suffix and the end of the prefix minus one. So like, if the prefix ends at i and the suffix starts at j, then the removable substring is i+1 to j-1, which has length (j-1 - (i+1) +1) = j -i -1. Wait, right, because the substring from i+1 to j-1 is (j-1 - (i+1) +1) = j - i -1.

So the plan is: precompute for each position in t, the earliest indices in s where each character of t can be matched. Similarly, precompute the latest indices in s where each character of t can be matched. Then, the maximum removable substring would be between the end of a t's prefix (say up to i in t) and the start of a t's suffix (starting from i+1 in t). The maximum difference between the latest start of the next part and the earliest end of the previous part minus one.

Wait, maybe let's break it down.

Let's say we have two arrays:

- left[i] is the earliest index in s where the first i characters of t are a subsequence. So left[0] = -1 (since no characters are taken), left[1] is the first occurrence of t[0], etc.

- right[i] is the latest index in s where the last i characters of t are a subsequence. So right[0] would be len(s), right[1] is the last occurrence of t[-1], etc.

Then, for each possible split of t into a prefix and suffix, like the first k characters and the remaining m -k characters (where m is the length of t), we can find the left[k] and right[m -k], and the removable region is between left[k] and right[m -k]. The maximum possible length is (right_part_start - left_part_end - 1). So for each k from 0 to m (inclusive), we compute this and take the maximum.

So the steps are:

1. Precompute the left array.

To compute left[i], for each character in t up to i-1, find the earliest positions in s. For example, for left[0], it's -1. For left[1], find the first occurrence of t[0]. For left[2], find the next occurrence of t[1] after left[1], etc.

This can be done by iterating through s once and tracking the current position in t. As we go through each character in s, whenever it matches the current t character, we increment the current t index and record the position in left. So left[i] is the position in s where the i-th character of t is matched.

Similarly for the right array. For the right array, right[i] represents the position in s where the i-th character from the end of t is matched. So for right[1], it's the last occurrence of t[-1]. For right[2], it's the last occurrence of t[-2] before the position of right[1], etc.

So how to compute right:

Start from the end of s and iterate backwards. For each character in t in reverse order, track where they are found. So for right[0] = len(s). Then, for right[1], find the last occurrence of t[-1]. For right[2], find the last occurrence of t[-2] before right[1], etc.

Once left and right arrays are computed, then for each possible split k (from 0 to m), we can take the left[k] (the end of the prefix) and the right[m -k] (the start of the suffix). The removable substring is the characters between left[k] +1 and right[m -k] -1. The length would be (right[m -k] -1) - (left[k] +1) +1 = right[m -k] - left[k] -1.

Wait, the length of the substring from a to b inclusive is (b -a +1). So if the substring starts at left[k] +1 and ends at right[m -k] -1, then the length is (right[m -k] -1) - (left[k] +1) +1 = right[m -k] - left[k] -1 -1 +1? Wait no, let's calculate:

start = left[k] + 1

end = right[m -k] -1

length = end - start +1 = (right[m -k] -1) - (left[k] +1) +1 = right[m -k] - left[k] -1.

Yes. So for each k, the maximum possible length is right[m -k] - left[k] -1. We need to take the maximum over all possible k from 0 to m.

So the algorithm steps:

- Compute left array (size m+1), where left[k] is the earliest position in s where the first k characters of t are matched.

- Compute right array (size m+1), where right[k] is the latest position in s where the last k characters of t are matched.

- For each k in 0 to m (inclusive), check if left[k] is less than right[m -k]. If so, then the length is right[m -k] - left[k] -1. We need to find the maximum of all such possible lengths.

Now, let's think about how to compute left and right arrays.

For left:

Initialize left[0] = -1.

current_pos = 0 in t.

Then, iterate through each character in s:

for i in range(len(s)):

    if current_pos < len(t) and s[i] == t[current_pos]:

        left[current_pos + 1] = i

        current_pos += 1

Once current_pos reaches len(t), break.

But what if t is longer than s? But the problem states that t is a subsequence of s, so t can't be longer. So no problem.

Similarly for right array:

Initialize right[0] = len(s).

current_pos = len(t) -1.

Iterate through s in reverse:

for i in reversed(range(len(s))):

    if current_pos >=0 and s[i] == t[current_pos]:

        right[len(t) - current_pos] = i

        current_pos -=1

Once current_pos is -1, break.

Wait, let's see. For right array:

We need to track how many characters from the end of t we've matched. For example, right[1] is the position of the last occurrence of t[-1]. right[2] is the position of the last occurrence of t[-2] before that, etc.

So for the right array:

Initialize right[0] = len(s).

current_pos = len(t) -1 (since we start from the end of t).

We loop i from len(s)-1 down to 0:

if s[i] matches t[current_pos], then we set right[k] = i, where k is (len(t) - current_pos). Because when current_pos is len(t)-1 (the last character), then k is 1. Then current_pos decreases by 1, and when we find the next character (t[-2]), k becomes 2, etc.

Once current_pos <0, we can stop.

So after processing, right[k] gives the latest position where the last k characters of t are matched.

Once we have left and right arrays filled, then for each possible split k (0 <= k <= m), we can check the possible length.

For example, if k=0, then the entire t is matched by the suffix. So left[0] is -1. The suffix part is m characters (the entire t), so right[m] is the position where the last m characters (the entire t) start. Then the removable substring is from 0 to right[m] -1, which would be right[m] - left[0] -1 = right[m] - (-1) -1 = right[m]. But wait, the entire prefix is 0 characters, and the suffix is m characters, so the substring to remove is everything between left[0] (which is -1) and right[m] (the start of the suffix). The substring would be from 0 to right[m]-1, length right[m] - 0 + 0? Wait, perhaps the formula is correct.

Let me take the first example:

Sample input 1:

s = bbaba, t=bb.

So t's left array:

left[0] = -1

left[1] is the first 'b' in s. s is indexes 0,1,2,3,4: 'b','b','a','b','a'. So first character of t is 'b' at 0. left[1] =0.

Then left[2] is the next 'b' after 0. So next is index 1. So left[2] =1.

So left array for k=2 is 1.

Right array for t's two characters:

right[0] =5 (len(s) is 5, since s is 'bbaba').

We start from current_pos=1 (t is 'b','b').

We iterate s in reverse:

i=4: 'a' doesn't match t[1] ('b').

i=3: 'b' matches. So right[1] =3. current_pos becomes 0.

i=2: 'a' no.

i=1: 'b' matches t[0]. So right[2] =1. current_pos becomes -1. Stop.

So right array is:

right[0] =5

right[1] =3 (position of the last 'b' in t)

right[2] =1 (position of the first 'b' in t, since the suffix of 2 characters is 'bb' which starts at 1 and ends at 3? Wait, maybe I'm getting confused.

Wait, for the right array:

right[1] is the position where the last 1 character of t is matched. t is 'bb', so the last 1 character is the last 'b', which is at index 3 in s.

right[2] is the position where the last 2 characters of t are matched. So for 'bb', the first 'b' must be before the second 'b'. So the last occurrence of 'bb' as a subsequence in s is when the first 'b' is at index 1 and the second at 3. So the right array for 2 would be 1 (the earliest index of the first 'b' in the pair).

Wait, the right array for k=2 (the entire t) is the earliest index of the first 'b' in the pair. Because when we build the right array, we start from the end of s and look for the last 'b' first. Then look for the previous 'b' before that.

So in the example, the right array for k=2 is 1, which is the index of the first 'b' in s. Then, the suffix part is the entire t (k=2), so the right array for k=2 is 1. Hmm, but how does that fit into the formula.

Wait, when we compute for k=0 (the entire t is the suffix part), then the split is 0 in the left (so left[0] is -1) and right[2] (since m is 2, so m -k=2). So the removable length is right[2] - left[0] -1 = 1 - (-1) -1 = 1. But the sample output is 3. Wait, maybe I'm misunderstanding the split.

Wait the split is between the first k characters of t (prefix) and the remaining m -k (suffix). So when k=0, all of t is in the suffix. So the left part is nothing (left[0] is -1), and the right part is the entire t (so right[2] is the position where the entire t is matched as a suffix). The substring to remove is the part between left[0] (-1) and the start of the suffix (right[2]). So the removable substring is from 0 to right[2]-1. The length is right[2] -1 -0 +1 = right[2]. For example, if right[2] is 1, then the substring is 0 to 0 (length 1). But the sample output is 3.

Hmm, perhaps I made a mistake in the right array calculation.

Wait, let's re-examine the sample input 1.

Sample 1:

s = "bbaba" (indices 0,1,2,3,4)

t = "bb"

left array:

left[0] = -1

left[1] = 0 (first 'b')

left[2] = 1 (second 'b' in s[1])

right array:

We are looking for the latest positions.

For right[1], the last 'b' in s is at index 3.

For right[2], the first 'b' must be before index 3. The latest possible 'b' is at index 1 (since s[1] is 'b' and then s[3] is 'b').

So right[2] is 1.

So when k=0, the left is -1, and the right is right[2 -0] = right[2] =1. So the removable substring is from left[0]+1=0 to right[2]-1=0. That's the substring [0,0], which has length 1. But the sample output is 3. So how does this approach get the correct answer?

Wait, the sample output is 3. The correct answer for sample 1 is 3. Let's see how that comes.

In sample 1, the optimal is to remove the substring from index 1 to 3 (the substring "ba b", but wait, indexes 1 to 3 would be s[1] is 'b', s[2] 'a', s[3] 'b'? So substring "bab" of length 3.

But how does this fit into the formula.

Wait, when we split t into k=1 and m-k=1. So left[k=1] is 0 (the first 'b'), and right[1] is 3 (the last 'b'). Then the removable substring is between left[1] (0) and right[1] (3). The substring is from 0+1=1 to 3-1=2. That's indices 1 to 2, length 2. Wait, no. Wait the formula says the length is right[m -k] - left[k] -1. For k=1, m is 2. m -k =1. So right[1] is 3. left[1] is 0. 3-0-1 =2. But the sample answer is 3. So perhaps this approach is not capturing the correct scenario.

Hmm, this suggests that the approach is not correct, or that I have a mistake in the way I'm building the left and right arrays.

Wait, let's re-examine the sample 1. The correct answer is 3. So the maximum substring that can be removed is 3 characters long.

In the sample, after removing the substring from index 1 to 3 (length 3), the remaining s is "b" + "a" (indices 0 and 4). So the original s is "bbaba". After removing 1-3, we have "b" + "a" = "ba". But t is "bb", which is a subsequence of "ba"? Wait, no. "ba" doesn't have two 'b's. So that's not possible. Wait what's the correct scenario?

Wait, sample input 1's output is 3. Let's think again. How can we remove a substring of length 3 so that t remains a subsequence.

Original s is b b a b a.

Suppose we remove the substring starting at index 1 (inclusive) to index 3 (inclusive): "b a b". So the remaining string is "b" (from index 0) + "a" (index4). So the new s is "ba". But t is "bb", which is not a subsequence. So that can't be right.

Wait maybe I have a misunderstanding of the sample. Let's recheck the sample input 1.

Sample input 1:

Input:

bbaba

bb

Output:3.

So the answer is 3. So which substring is removed?

The correct removal must leave t as a subsequence.

Possible solution: remove the substring from index 2 to 4 (characters 'a', 'b', 'a'). The remaining s is "bb", which is exactly t. So yes, the length is 3.

Ah right. So the substring is indices 2-4. So after removing that, s becomes "bb", which has t as a subsequence. So how does this fit into the left and right approach.

In this case, the left part is the first two characters of t (but since t has two 'b's), the left[2] is 1 (the second 'b' at index1). The right part is the remaining 0 characters (since m-k is 0 when k=2). So right[0] is len(s)=5. So the removable substring is between left[2]+1=2 and right[0]-1=4 (since 5-1=4). So the substring is from 2 to4, which is length 4-2 +1=3. So in this case, when k=2, the formula gives right[0] - left[2] -1 =5 -1 -1=3, which is the correct length. So the maximum is achieved when k=2.

So the approach works here.

So why wasn't that considered in the initial approach? Because when k is 2, m -k is 0. So right[0] is 5. So for k=2, the length is 5-1-1=3.

So the maximum is achieved at k=2.

So the left array is:

left[0] = -1

left[1] =0

left[2] =1

right array:

right[0] =5

right[1] =3

right[2] =1.

Wait no, for right array:

right[1] is the position where the last 1 character is matched (the last 'b' in t's last 1 character). So that's index3.

right[2] is the position where the last 2 characters are matched, which would be the first 'b' in the pair. So in s, the first 'b' is at0, second at1. But when building the right array, we start from the end. So for t's two 'b's:

Looking for the last occurrence of the second 'b' (which is t[1] = 'b'). So in s, the last 'b' is at index3. Then, looking for the last occurrence of 'b' (t[0]) before that. The last 'b' before index3 is at index1. So right[2] is1.

So right array for k=0 is5, k=1 is3, k=2 is1.

So when k=2 (split into 2 and 0), left[2] is1, right[0] is5. So the length is5 -1 -1=3.

So that's correct.

So the approach is to loop through all possible k from 0 to m (inclusive) and compute the maximum value of (right[m-k] - left[k] -1).

Now, the next step is to implement this.

But how to handle cases where left[k] is not found (but according to the problem statement, t is a subsequence of s, so left[m] must be found, and similarly for right[m].

So now, the code steps:

Read s and t.

Compute left array.

Compute right array.

Then, for each k in 0 to len(t), calculate (right[len(t)-k] - left[k] -1). Take the maximum of these.

So in code:

m = len(t)

left = [-1] * (m+1)

left[0] = -1

current = 0

for i in range(len(s)):

    if current < m and s[i] == t[current]:

        current +=1

        left[current] = i

right = [len(s)] * (m+1)

current = m-1

for i in reversed(range(len(s))):

    if current >=0 and s[i] == t[current]:

        right[m - current] = i

        current -=1

max_len = 0

for k in range(m+1):

    if left[k] < right[m -k]:

        max_len = max(max_len, right[m -k] - left[k] -1)

print(max_len)

Yes.

But what if m is 0? But according to the problem statement, t has at least 1 character.

Wait the constraints say t has at least 1 character. So no problem.

Now, let's test the code with sample input 1.

Sample 1:

s = "bbaba", len=5

t = "bb", len=2.

left array:

left[0] =-1

left[1] =0 (first 'b')

left[2] =1 (second 'b' at index1)

right array:

right[0] =5

right[1] =3 (last 'b' is at index3)

right[2] =1 (the first 'b' at index1)

For k=0:

right[2] =1. left[0] =-1. 1 - (-1) -1=1.

k=1: right[1] =3. left[1] =0. 3-0-1=2.

k=2: right[0]=5. left[2]=1. 5-1-1=3.

So the maximum is 3. Which matches the sample.

Sample 2:

Input:

baaba

ab

So s is 'b','a','a','b','a'.

t is 'a','b'.

left array:

left[0] =-1.

current=0.

s[0] is 'b' which is t[0] (a?) No. So left[0] remains -1.

s[1] is 'a' which matches t[0]. So left[1] =1. current becomes1.

s[2] is 'a' not 'b' (t[1] is 'b'). s[3] is 'b' matches. left[2] =3. current becomes2. So left array is [-1,1,3].

right array:

t is 'ab'. current starts at1 (index of 'b' in t).

We loop s in reverse:

s[4] is 'a' which is t[1] (current=1)? No. t[1] is 'b'.

s[3] is 'b' matches t[1]. So right[1] =3. current becomes0.

Then, look for 'a' (t[0]) before index3.

s[2] is 'a' matches t[0]. So right[2] =2. current becomes-1.

So right array is:

right[0]=5 (len(s) is5).

right[1]=3.

right[2]=2.

Now, for k in 0,1,2:

k=0: right[2] =2. left[0] =-1. 2 - (-1) -1= 2.

k=1: right[1] =3. left[1] =1. 3-1-1=1.

k=2: right[0] =5. left[2] =3. 5-3-1=1.

So maximum is 2. Which matches the sample output.

Another sample: input 3 is s=abcde and t=abcde. So the only way to remove is nothing. So the maximum is0.

In this case, left array is [-1,0,1,2,3,4]. right array is [5,4,3,2,1,0]. For k=5, m=5. So m -k =0. So right[0]=5. left[5] =4. 5-4-1=0. So the maximum is0.

Another sample: input4:

s=asdfasdf

t=fasd

The sample output is3.

But regardless, the code should compute correctly.

So the code seems to handle all cases.

Now, considering the constraints: s and t can be up to 2e5 in length. The code runs in O(n + m) time, which is acceptable.

The left and right arrays are built in O(n) each. Then, the loop over m is O(m), which is acceptable.

Now, in Python, we need to implement this efficiently.

Edge cases:

- When t is exactly s: then the only possible removable substring is length 0.

- When t is empty: but according to the problem statement, t is at least 1.

Another case: when all of t is in the prefix. For example, s is t + some characters. Then the maximum removable substring would be the characters after the prefix.

Wait, let's see. For example, s = "abcde", t = "ab". The left array would have left[2] =1. The right array for m -k=0 (since k=2), right[0] is5. So the length is5 -1-1=3. Which is correct (the substring from 2 to4).

So code works.

Another case: when t is a single character. For example, s="aaaaa", t="a". Then left[1] =0. right[1] =4. So for k=0: right[1] - (-1) -1=4+1-1=4. For k=1: right[0] =5. 5 -0 -1=4. So maximum is4.

Which is correct, since you can remove any substring that leaves one 'a' in the remaining s.

So the code works.

Now, let's code this in Python.

Read s and t.

Compute left array.

Then compute right array.

Then iterate through k from0 to len(t), compute the maximum.

Now, code:

Read s and t:

Testing against sample input 1.

```python
def main(input_stream, output_stream):
    s = input_stream.readline().rstrip("\n").strip()

    t = input_stream.readline().rstrip("\n").strip()

    m = len(t)

    n = len(s)

    left = [-1]*(m+1)

    current =0

    for i in range(n):

        if current < m and s[i] == t[current]:

            current +=1

            left[current] = i

    right = [n]*(m+1)

    current = m-1

    for i in reversed(range(n)):

        if current >=0 and s[i] == t[current]:

            # the number of characters matched from the end is (m - current)

            right[m - current] = i

            current -=1

    max_len =0

    for k in range(m+1):

        # t is split into first k and last m-k characters

        # right part is m-k characters from the end

        # right[m-k] is the earliest index for the suffix part

        # left[k] is the latest index for the prefix part

        # if left[k] < right[m-k], then the removable region is between them

        if left[k] < right[m -k]:

            max_len = max(max_len, right[m -k] - left[k] -1)

    print(max_len, file=output_stream)



def test():
    import io

    TEST_CASES = [
        {
            "input": \
"""\
baaba
ab
""",
            "output": \
"""\
2
""",
        }, 
    ]

    for i, test_case in enumerate(TEST_CASES):
        in_stream = io.StringIO(test_case["input"])
        expected_output = test_case["output"].rstrip()

        out_stream = io.StringIO()
        main(in_stream, out_stream)
        real_output = out_stream.getvalue().rstrip()

        assert real_output == expected_output, \
            f'Test case {i} failed.\nExpected: {expected_output!r}\nGot: {real_output!r}'

    print('Tests passed 😎')


if __name__ == '__main__':
    test()


```

<RUN_SNIPPET>
```output
Tests passed 😎

```

Testing against sample input 2.

```python
def main(input_stream, output_stream):
    s = input_stream.readline().rstrip("\n").strip()

    t = input_stream.readline().rstrip("\n").strip()

    m = len(t)

    n = len(s)

    left = [-1]*(m+1)

    current =0

    for i in range(n):

        if current < m and s[i] == t[current]:

            current +=1

            left[current] = i

    right = [n]*(m+1)

    current = m-1

    for i in reversed(range(n)):

        if current >=0 and s[i] == t[current]:

            # the number of characters matched from the end is (m - current)

            right[m - current] = i

            current -=1

    max_len =0

    for k in range(m+1):

        # t is split into first k and last m-k characters

        # right part is m-k characters from the end

        # right[m-k] is the earliest index for the suffix part

        # left[k] is the latest index for the prefix part

        # if left[k] < right[m-k], then the removable region is between them

        if left[k] < right[m -k]:

            max_len = max(max_len, right[m -k] - left[k] -1)

    print(max_len, file=output_stream)



def test():
    import io

    TEST_CASES = [
        {
            "input": \
"""\
abcde
abcde
""",
            "output": \
"""\
0
""",
        }, 
    ]

    for i, test_case in enumerate(TEST_CASES):
        in_stream = io.StringIO(test_case["input"])
        expected_output = test_case["output"].rstrip()

        out_stream = io.StringIO()
        main(in_stream, out_stream)
        real_output = out_stream.getvalue().rstrip()

        assert real_output == expected_output, \
            f'Test case {i} failed.\nExpected: {expected_output!r}\nGot: {real_output!r}'

    print('Tests passed 😎')


if __name__ == '__main__':
    test()


```

<RUN_SNIPPET>
```output
Tests passed 😎

```

So the code works.

Thus, the code should be correct.
</think>

```python
s = input().strip()
t = input().strip()
m = len(t)
n = len(s)

left = [-1] * (m + 1)
current = 0
for i in range(n):
    if current < m and s[i] == t[current]:
        current += 1
        left[current] = i

right = [n] * (m + 1)
current = m - 1
for i in reversed(range(n)):
    if current >= 0 and s[i] == t[current]:
        right[m - current] = i
        current -= 1

max_len = 0
for k in range(m + 1):
    if left[k] < right[m - k]:
        max_len = max(max_len, right[m - k] - left[k] - 1)

print(max_len)
```
